ConNF/Counting/StrongSupport.lean
@@ -36,11 +36,12 @@ inductive Precedes : Address β → Address β → Prop
 
 @[mk_iff]
 structure Strong (S : Support β) : Prop where
+  /-- TODO: We can simplify this statement now that we've removed the extra inequalities. -/
   interferes {i₁ i₂ : κ} (hi₁ : i₁ < S.max) (hi₂ : i₂ < S.max)
     {A : ExtendedIndex β} {N₁ N₂ : NearLitter}
     (h₁ : S.f i₁ hi₁ = ⟨A, inr N₁⟩) (h₂ : S.f i₂ hi₂ = ⟨A, inr N₂⟩)
     {a : Atom} (ha : Interferes a N₁ N₂) :
-    ∃ (j : κ) (hj : j < S.max), j < i₁ ∧ j < i₂ ∧ S.f j hj = ⟨A, inl a⟩
+    ∃ (j : κ) (hj : j < S.max), S.f j hj = ⟨A, inl a⟩
   precedes {i : κ} (hi : i < S.max) (c : Address β) (hc : Precedes c (S.f i hi)) :
     ∃ (j : κ) (hj : j < S.max), j < i ∧ S.f j hj = c
 
@@ -260,14 +261,7 @@ theorem strongSupport_strong {s : Set (Address β)} (hs : Small s) : (strongSupp
     rw [hN₁] at hi₁'
     rw [hN₂] at hi₂'
     have := interferes_mem_strongClosure s A a N₁ N₂ ha hi₁' hi₂'
-    obtain ⟨j, hj, hc⟩ := exists_of_mem_strongClosure _ _ this
-    refine ⟨j, hj, ?_, ?_, hc⟩
-    · refine lt_of_strongSupportRel hs hj hi₁ ?_
-      rw [hc, hN₁]
-      exact StrongSupportRel.atom _ _ _ _
-    · refine lt_of_strongSupportRel hs hj hi₂ ?_
-      rw [hc, hN₂]
-      exact StrongSupportRel.atom _ _ _ _
+    exact exists_of_mem_strongClosure _ _ this
   · intro i hi c hc
     have hi' := mem_of_strongSupport_f_eq hs hi
     have := precedes_mem_strongClosure s hc hi'
@@ -345,8 +339,8 @@ theorem Strong.smul [LeLevel β] {S : Support β} (hS : S.Strong) (ρ : Allowabl
     have := hS.interferes hi₁ hi₂
         (N₁ := (Allowable.toStructPerm ρ A)⁻¹ • N₁) (N₂ := (Allowable.toStructPerm ρ A)⁻¹ • N₂)
         ?_ ?_ (A := A) (a := (Allowable.toStructPerm ρ A)⁻¹ • a) this
-    · obtain ⟨j, hj, hj₁, hj₂, h⟩ := this
-      refine ⟨j, hj, hj₁, hj₂, ?_⟩
+    · obtain ⟨j, hj, h⟩ := this
+      refine ⟨j, hj, ?_⟩
       rw [Enumeration.smul_f, h, Allowable.smul_address, smul_inl, smul_inv_smul]
     · rw [Enumeration.smul_f, smul_eq_iff_eq_inv_smul] at hN₁
       rw [hN₁, Allowable.smul_address, map_inv, Tree.inv_apply, smul_inr]
@@ -379,16 +373,6 @@ theorem before_carrier (S : Support β) (i : κ) (hi : i < S.max) :
     exact ⟨j, _, hj, rfl⟩
   · rintro ⟨j, hj₁, hj₂, rfl⟩
     exact ⟨j, hj₂, rfl⟩
-
-theorem before_strong (S : Support β) (i : κ) (hi : i < S.max) (hS : S.Strong) :
-    (S.before i hi).Strong := by
-  constructor
-  · intro i₁ i₂ hi₁ hi₂ A N₁ N₂ hN₁ hN₂ a ha
-    obtain ⟨j, hj, hj₁, hj₂, h⟩ := hS.interferes (hi₁.trans hi) (hi₂.trans hi) hN₁ hN₂ ha
-    exact ⟨j, hj₁.trans hi₁, hj₁, hj₂, h⟩
-  · intro j hj c hc
-    obtain ⟨k, hk₁, hk₂, h⟩ := hS.precedes (hj.trans hi) c hc
-    exact ⟨k, hk₂.trans hj, hk₂, h⟩
 
 @[simp]
 theorem before_smul [LeLevel β] (S : Support β) (i : κ) (hi : i < S.max) (ρ : Allowable β) :
@@ -582,18 +566,10 @@ theorem comp_strong {γ : Λ} (S : Support β) (A : Path (β : TypeIndex) γ) (h
     have h₂ := decomp_spec hS' hi₂
     rw [hN₁] at h₁
     rw [hN₂] at h₂
-    obtain ⟨j, hj, hj₁, hj₂, h⟩ := hS.interferes _ _ h₁ h₂ ha
-    refine ⟨j, ?_, ?_, ?_, ?_⟩
+    obtain ⟨j, hj, h⟩ := hS.interferes _ _ h₁ h₂ ha
+    refine ⟨j, ?_, ?_⟩
     · rw [comp_max_eq_of_canComp hS']
       exact hj
-    · rw [compIndex] at hj₁
-      split_ifs at hj₁ with hj'
-      · exact hj₁
-      · exact (not_lt_leastCompIndex hS' j ⟨hj, ⟨B, inl a⟩, h⟩ hj₁).elim
-    · rw [compIndex] at hj₂
-      split_ifs at hj₂ with hj'
-      · exact hj₂
-      · exact (not_lt_leastCompIndex hS' j ⟨hj, ⟨B, inl a⟩, h⟩ hj₂).elim
     · rw [comp_f_eq]
       exact comp_decomp_eq hS' hj h
   · intro i hi c hc
